steel/Zeta.Steel.VerifierTypes.fsti
@@ -13,14 +13,35 @@ val thread_state_t
 val thread_id (t:thread_state_t)
   : tid
 
-val thread_state_inv (t:thread_state_t) ([@@@smt_fallback] m:M.thread_state_model)
+val thread_state_inv_core (t:thread_state_t)
+                          ([@@@smt_fallback] m:M.thread_state_model)
   : vprop
+
+let tsm_entries_invariant (tsm:M.thread_state_model) =
+    not tsm.failed ==>
+    tsm == M.verify_model (M.init_thread_state_model tsm.thread_id)
+                          tsm.processed_entries
+
+val thread_state_inv (t:thread_state_t)
+                     ([@@@smt_fallback] m:M.thread_state_model)
+  : vprop
+
+val intro_thread_state_inv (#o:_)
+                           (#tsm:M.thread_state_model)
+                           (t:thread_state_t)
+  : STGhost unit o
+    (thread_state_inv_core t tsm)
+    (fun _ -> thread_state_inv t tsm)
+    (requires
+      thread_id t == tsm.thread_id /\
+      tsm_entries_invariant tsm)
+    (ensures fun _ -> True)
 
 val elim_thread_state_inv (#o:_) (#tsm:M.thread_state_model) (t:thread_state_t)
   : STGhost unit o
     (thread_state_inv t tsm)
-    (fun _ -> thread_state_inv t tsm)
+    (fun _ -> thread_state_inv_core t tsm)
     (requires True)
     (ensures fun _ ->
-      tsm == M.verify_model (M.init_thread_state_model (thread_id t))
-                            tsm.processed_entries)
+      thread_id t == tsm.thread_id /\
+      tsm_entries_invariant tsm)
