steel/Zeta.Steel.Verifier.fsti
@@ -20,12 +20,10 @@ module TLM = Zeta.Steel.ThreadLogMap
 
 #push-options "--ide_id_info_off"
 
-val create (tid:tid)
-  : STT thread_state_t
-    emp
-    (fun t -> thread_state_inv t (M.init_thread_state_model tid))
-
-
+// val create (tid:tid)
+//   : STT thread_state_t
+//     emp
+//     (fun t -> thread_state_inv t (M.init_thread_state_model tid))
 
 val spec_parser_log : P.spec_parser (Seq.seq log_entry)
 
