steel/Zeta.Steel.VerifierSteps.fst
@@ -1,0 +1,1389 @@
+module Zeta.Steel.VerifierSteps
+friend Zeta.Steel.VerifierTypes
+open Zeta.Steel.VerifierTypes
+open FStar.Ghost
+open Steel.ST.Util
+module G = Steel.ST.GhostReference
+module R = Steel.ST.Reference
+module A = Steel.ST.Array
+module TLM = Zeta.Steel.ThreadLogMap
+open Zeta.Steel.ApplicationTypes
+module U8 = FStar.UInt8
+module U16 = FStar.UInt16
+module U32 = FStar.UInt32
+module U64 = FStar.UInt64
+open Zeta.Steel.FormatsManual
+open Zeta.Steel.Util
+module T = Zeta.Steel.FormatsManual
+module M = Zeta.Steel.ThreadStateModel
+module AEH = Zeta.Steel.AggregateEpochHashes
+module Cast = FStar.Int.Cast
+open Zeta.Steel.EpochHashes
+module KU = Zeta.Steel.KeyUtils
+module EH = Zeta.Steel.EpochHashes
+module HA = Zeta.Steel.HashAccumulator
+#push-options "--ide_id_info_off"
+#push-options "--query_stats --fuel 0 --ifuel 1"
+
+let as_u32 (s:U16.t) : U32.t = Cast.uint16_to_uint32 s
+
+
+let fail (#tsm:M.thread_state_model)
+         (t:thread_state_t)
+  : STT unit
+    (thread_state_inv_core t tsm)
+    (fun _ -> thread_state_inv_core t (M.fail tsm))
+  = R.write t.failed true
+
+let fail_as (#tsm:M.thread_state_model)
+            (t:thread_state_t)
+            (tsm':M.thread_state_model)
+  : ST bool
+    (thread_state_inv_core t tsm)
+    (fun b -> thread_state_inv_core t (update_if b tsm tsm'))
+    (requires tsm' == M.fail tsm)
+    (ensures fun _ -> True)
+  = R.write t.failed true;
+    let b = true in
+    intro_thread_state_inv_core (update_if b tsm tsm') t;
+    return b
+
+////////////////////////////////////////////////////////////////////////////////
+//create
+////////////////////////////////////////////////////////////////////////////////
+
+#push-options "--fuel 1"
+let create (tid:tid)
+  : STT thread_state_t
+    emp
+    (fun t -> thread_state_inv t (M.init_thread_state_model tid))
+  = let failed = R.alloc false in
+    let store : vstore = A.alloc None (as_u32 store_size) in
+    let clock = R.alloc 0uL in
+    let epoch_hashes = EpochMap.create 64ul M.init_epoch_hash in
+    let last_verified_epoch = R.alloc 0ul in
+    let processed_entries : G.ref (Seq.seq log_entry) = G.alloc Seq.empty in
+    let app_results : G.ref M.app_results = G.alloc Seq.empty in
+    let serialization_buffer = A.alloc 0uy 4096ul in
+    let tsm = M.init_thread_state_model tid in
+    let t : thread_state_t = {
+        thread_id = tid;
+        failed;
+        store;
+        clock;
+        epoch_hashes;
+        last_verified_epoch;
+        processed_entries;
+        app_results;
+        serialization_buffer
+    } in
+    intro_exists _ (array_pts_to serialization_buffer);
+    assert (tsm == M.verify_model tsm Seq.empty);
+    intro_pure (tsm_entries_invariant (M.init_thread_state_model tid) /\
+                t.thread_id == tsm.thread_id);
+    rewrite (R.pts_to failed _ _ `star`
+             array_pts_to store _ `star`
+             R.pts_to clock _ _ `star`
+             EpochMap.full_perm epoch_hashes _ _ `star`
+             R.pts_to last_verified_epoch _ _ `star`
+             G.pts_to processed_entries _ _ `star`
+             G.pts_to app_results _ _ `star`
+             exists_ (array_pts_to serialization_buffer) `star`
+             pure (tsm_entries_invariant (M.init_thread_state_model tid) /\
+                   t.thread_id == tsm.thread_id)
+            )
+            (thread_state_inv t (M.init_thread_state_model tid));
+    return t
+#pop-options
+
+////////////////////////////////////////////////////////////////////////////////
+//vaddm
+////////////////////////////////////////////////////////////////////////////////
+
+let madd_to_store_split (#tsm:M.thread_state_model)
+                        (t:thread_state_t)
+                        (s:T.slot)
+                        (k:key)
+                        (v:T.value)
+                        (s':T.slot)
+                        (d:bool)
+                        (d2:bool)
+  : STT unit
+    (thread_state_inv_core t tsm)
+    (fun _ -> thread_state_inv_core t (M.madd_to_store_split tsm s k v s' d d2))
+  = let b = (T.is_value_of k v) in
+    if not b
+    then (fail t; return ())
+    else (
+      let ropt = A.read t.store (as_u32 s) in
+      let ropt' = A.read t.store (as_u32 s') in
+      match ropt with
+      | Some _ -> fail t; return ()
+      | _ ->
+        match ropt' with
+        | None -> fail t; return ()
+        | Some r' ->
+          let p = (s', d) in
+          let s2_opt = M.child_slot r' d in
+          match s2_opt with
+          | None -> fail t; return ()
+          | Some s2 ->
+            let r2opt = A.read t.store (as_u32 s2) in
+            match r2opt with
+            | None -> fail t; return ()
+            | Some r2 ->
+              let e = M.mk_entry_full k v M.MAdd None None (Some p) in
+              let e = M.update_child e d2 s2 in
+              let e' = M.update_child r' d s in
+              let p2new = s2, d2 in
+              let e2 = M.update_parent_slot r2 p2new in
+              A.write t.store (as_u32 s) (Some e);
+              A.write t.store (as_u32 s') (Some e');
+              A.write t.store (as_u32 s2) (Some e2);
+              return ())
+
+let madd_to_store (#tsm:M.thread_state_model)
+                  (t:thread_state_t)
+                  (s:T.slot)
+                  (k:key)
+                  (v:T.value)
+                  (s':T.slot)
+                  (d:bool)
+  : STT unit
+    (thread_state_inv_core t tsm)
+    (fun _ -> thread_state_inv_core t (M.madd_to_store tsm s k v s' d))
+  = let b = (T.is_value_of k v) in
+    if not b
+    then (fail t; return ())
+    else (
+      let ropt = A.read t.store (as_u32 s) in
+      let ropt' = A.read t.store (as_u32 s') in
+      match ropt with
+      | Some _ -> fail t; return ()
+      | _ ->
+        match ropt' with
+        | None -> fail t; return ()
+        | Some r' ->
+          let new_entry : M.store_entry = {
+            key = k;
+            value = v;
+            add_method = M.MAdd;
+            l_child_in_store = None;
+            r_child_in_store = None;
+            parent_slot = Some (s', d)
+          } in
+          A.write t.store (as_u32 s) (Some new_entry);
+          let r' : M.store_entry =
+            if d
+            then { r' with l_child_in_store = Some s }
+            else { r' with r_child_in_store = Some s }
+          in
+          A.write t.store (as_u32 s') (Some r');
+          return ()
+    )
+
+let entry_points_to_some_slot (r:M.store_entry)
+                              (d:bool)
+  : bool
+  = if d
+    then Some? (r.l_child_in_store)
+    else Some? (r.r_child_in_store)
+
+let update_value (#tsm:M.thread_state_model)
+                 (t:thread_state_t)
+                 (s:slot { M.has_slot tsm s })
+                 (r:value { T.is_value_of (M.key_of_slot tsm s) r})
+  : STT unit
+    (thread_state_inv_core t tsm)
+    (fun _ -> thread_state_inv_core t (M.update_value tsm s r))
+  = let Some v = A.read t.store (as_u32 s) in
+    A.write t.store (as_u32 s) (Some ({v with M.value = r}));
+    ()
+
+let vaddm (#tsm:M.thread_state_model)
+          (t:thread_state_t)
+          (s s':slot_id)
+          (r:T.record)
+  : STT bool
+    (thread_state_inv_core t tsm)
+    (fun b -> thread_state_inv_core t (update_if b tsm (M.vaddm tsm s s' r)))
+  = let b = not (M.check_slot_bounds s)
+          || not (M.check_slot_bounds s') in
+    if b then (fail t; return true)
+    else (
+      let gk, gv = r in
+      let ropt = A.read t.store (as_u32 s') in
+      match ropt with
+      | None -> (fail t; return true)
+      | Some r' ->
+        let k' = M.to_base_key r'.key in
+        let v' = r'.value in
+        let k = M.to_base_key gk in
+        (* check k is a proper desc of k' *)
+        if not (KU.is_proper_descendent k k')
+        then (fail t; return true)
+        (* check store does not contain slot s *)
+        else (
+          let sopt = A.read t.store (as_u32 s) in
+          match sopt with
+          | Some _ -> fail t; return true
+          | _ ->
+             match M.to_merkle_value v' with
+             | None -> fail t; return true
+             | Some v' ->
+               let d = KU.desc_dir k k' in
+               let dh' = M.desc_hash_dir v' d in
+               let h = M.hashfn gv in //TODO: low-level hash
+               match dh' returns
+                     (STT bool
+                          (thread_state_inv_core t tsm)
+                          (fun b -> thread_state_inv_core t (update_if b tsm (M.vaddm tsm s s' r))))
+               with
+               | T.Dh_vnone _ -> (* k' has no child in direction d *)
+                 (* first add must be init value *)
+                 if gv <> M.init_value gk
+                 then (let b = fail_as t _ in return b)
+                 else if entry_points_to_some_slot r' d
+                 then (let b = fail_as t _ in return b)
+                 else (
+                   madd_to_store t s gk gv s' d;
+                   let v'_upd = M.update_merkle_value v' d k h false in
+                   update_value t s' (T.MValue v'_upd);
+                   return true
+                 )
+               | T.Dh_vsome {T.dhd_key=k2; T.dhd_h=h2; T.evicted_to_blum = b2} ->
+                 if k2 = k
+                 then (
+                   if not (h2 = h && b2 = T.Vfalse)
+                   then (let b = fail_as t _ in return b)
+                   else if entry_points_to_some_slot r' d
+                   then (let b = fail_as t _ in return b)
+                   else (madd_to_store t s gk gv s' d;
+                         assert_ (thread_state_inv_core t (M.vaddm tsm s s' r));
+                         let b = true in
+//                         intro_thread_state_inv_core (update_if b tsm (M.vaddm tsm s s' p)) t;
+                         return b)
+                 )
+                 else if gv <> M.init_value gk
+                 then (let b = fail_as t _ in return b)
+                 (* check k2 is a proper desc of k *)
+                 else if not (KU.is_proper_descendent k2 k)
+                 then (let b = fail_as t _ in return b)
+                 else (
+                   let d2 = KU.desc_dir k2 k in
+                   let Some mv = M.to_merkle_value gv in
+                   let mv_upd = M.update_merkle_value mv d2 k2 h2 (b2=T.Vtrue) in
+                   let v'_upd = M.update_merkle_value v' d k h false in
+                   let b = entry_points_to_some_slot r' d in
+                   if b returns
+                     (STT bool
+                          (thread_state_inv_core t tsm)
+                          (fun b -> thread_state_inv_core t (update_if b tsm (M.vaddm tsm s s' r))))
+                   then (
+                     madd_to_store_split t s gk (MValue mv_upd) s' d d2;
+                     update_value t s' (MValue v'_upd);
+                     let b = true in
+                     return b
+                   )
+                   else (
+                     madd_to_store t s gk (MValue mv_upd) s' d;
+                     update_value t s' (MValue v'_upd);
+                     let b = true in
+                     return b
+                   )
+                 )))
+
+////////////////////////////////////////////////////////////////////////////////
+//vaddb
+////////////////////////////////////////////////////////////////////////////////
+
+let next (t:T.timestamp)
+  : option T.timestamp
+  = if FStar.UInt.fits (U64.v t + 1) 64
+    then Some (U64.add t 1uL)
+    else None
+
+let max (t0 t1:T.timestamp)
+  = let open U64 in
+    if t0 >=^ t1 then t0 else t1
+
+type htype =
+  | HAdd
+  | HEvict
+
+let update_hash (c:M.epoch_hash)
+                (r:T.record)
+                (t:T.timestamp)
+                (thread_id:T.thread_id)
+                (ht:htype)
+  : GTot M.epoch_hash
+  = match ht with
+    | HAdd -> { c with hadd = M.update_hash_value c.hadd r t thread_id }
+    | HEvict -> { c with hevict = M.update_hash_value c.hevict r t thread_id }
+
+let update_epoch_hash (tsm:M.thread_state_model)
+                      (e:M.epoch_id)
+                      (r:T.record)
+                      (ts:T.timestamp)
+                      (thread_id:T.thread_id)
+                      (ht:htype)
+   : M.thread_state_model
+  = let c = Map.sel tsm.epoch_hashes e in
+    {tsm with epoch_hashes =
+                   Map.upd tsm.epoch_hashes
+                      e
+                      (update_hash c r ts thread_id ht)}
+
+let maybe_update_epoch_hash (b:bool)
+                            (tsm:M.thread_state_model)
+                            (e:M.epoch_id)
+                            (r:T.record)
+                            (ts:T.timestamp)
+                            (thread_id:T.thread_id)
+                            (ht:htype)
+   : M.thread_state_model
+  = let c = Map.sel tsm.epoch_hashes e in
+    {tsm with epoch_hashes =
+                   Map.upd tsm.epoch_hashes
+                      e
+                      (update_if b c (update_hash c r ts thread_id ht))}
+
+let maybe_update_epoch_hash_equiv
+                          (b:bool)
+                          (tsm:M.thread_state_model)
+                          (e:M.epoch_id)
+                          (r:T.record)
+                          (ts:T.timestamp)
+                          (thread_id:T.thread_id)
+                          (ht:htype)
+  : Lemma (requires
+            Map.contains tsm.epoch_hashes e)
+          (ensures
+            maybe_update_epoch_hash b tsm e r ts thread_id ht ==
+            update_if b tsm (update_epoch_hash tsm e r ts thread_id ht))
+  = if b then ()
+    else assert (Map.equal tsm.epoch_hashes (Map.upd tsm.epoch_hashes e (Map.sel tsm.epoch_hashes e)))
+
+let unfold_epoch_hash_perm #o (k:M.epoch_id) (v:epoch_hashes_t) (c:M.epoch_hash)
+  : STGhostT unit o
+    (epoch_hash_perm k v c)
+    (fun _ ->
+      HA.ha_val v.hadd c.hadd `star`
+      HA.ha_val v.hevict c.hevict)
+  = rewrite (epoch_hash_perm k v c)
+            (HA.ha_val v.hadd c.hadd `star`
+             HA.ha_val v.hevict c.hevict)
+
+let fold_epoch_hash_perm #o
+                         (k:M.epoch_id)
+                         (v:epoch_hashes_t)
+                         (#had #hev:HA.hash_value_t)
+                         (c:M.epoch_hash)
+  : STGhost unit o
+    (HA.ha_val v.hadd had `star`
+     HA.ha_val v.hevict hev)
+    (fun _ -> epoch_hash_perm k v c)
+    (requires
+      c.hadd == had /\
+      c.hevict == hev)
+    (ensures fun _ -> True)
+  = rewrite (HA.ha_val v.hadd had `star`
+             HA.ha_val v.hevict hev)
+            (epoch_hash_perm k v c)
+
+
+let ha_add (#v:erased (HA.hash_value_t))
+           (ha:HA.ha)
+           (l:U32.t)
+           (#bs:erased bytes { U32.v l <= Seq.length bs /\ Seq.length bs <= HA.blake2_max_input_length })
+           (input:A.array U8.t)
+  : STT bool
+       (HA.ha_val ha v `star` array_pts_to input bs)
+       (fun b ->
+         array_pts_to input bs `star`
+         HA.ha_val ha (HA.maybe_aggregate_hashes b v
+                         (HA.hash_one_value (Seq.slice bs 0 (U32.v l)))))
+  = A.pts_to_length input _;
+    let x = HA.add ha input l in
+    return x
+
+#push-options "--z3rlimit_factor 2"
+let update_ht (#tsm:M.thread_state_model)
+              (t:thread_state_t)
+              (e:M.epoch_id)
+              (r:T.record)
+              (ts:T.timestamp)
+              (thread_id:T.thread_id)
+              (ht:htype)
+  : STT bool
+    (thread_state_inv_core t tsm)
+    (fun b -> thread_state_inv_core t (update_if b tsm (update_epoch_hash tsm e r ts thread_id ht)))
+  = let vopt = EpochMap.get t.epoch_hashes e in
+    match vopt with
+    | EpochMap.NotFound
+    | EpochMap.Fresh ->
+      rewrite (EpochMap.get_post _ _ _ _ _ vopt)
+              (EpochMap.full_perm t.epoch_hashes M.init_epoch_hash tsm.epoch_hashes);
+      return false
+
+    | EpochMap.Found v ->
+      rewrite (EpochMap.get_post _ _ _ _ _ vopt)
+              (EpochMap.perm t.epoch_hashes M.init_epoch_hash tsm.epoch_hashes (PartialMap.upd e v EpochMap.empty_borrows) `star`
+               EH.epoch_hash_perm e v (Map.sel tsm.epoch_hashes e));
+      unfold_epoch_hash_perm _ _ _;
+      let sr = {
+        record = r;
+        timestamp = ts;
+        thread_id = thread_id
+      } in
+      T.serialized_stamped_record_length sr;
+      let n = T.serialize_stamped_record 4096ul 0ul t.serialization_buffer sr in
+      let bs = elim_exists () in
+      elim_pure ( _ /\ _ /\ _ /\ _);
+      let ha = if ht = HAdd then v.hadd else v.hevict in
+      let b =
+        match ht
+              returns (STT bool
+                           (HA.ha_val v.hadd (Map.sel tsm.epoch_hashes e).hadd `star`
+                            HA.ha_val v.hevict (Map.sel tsm.epoch_hashes e).hevict `star`
+                            array_pts_to t.serialization_buffer bs
+                            )
+                           (fun b ->
+                             array_pts_to t.serialization_buffer bs `star`
+                             EH.epoch_hash_perm e v
+                              (update_if b (Map.sel tsm.epoch_hashes e)
+                                           (update_hash (Map.sel tsm.epoch_hashes e) r ts thread_id ht))))
+        with
+        | HAdd ->
+          let b = ha_add v.hadd n t.serialization_buffer in
+          fold_epoch_hash_perm e v
+               (update_if b (Map.sel tsm.epoch_hashes e)
+                            (update_hash (Map.sel tsm.epoch_hashes e) r ts thread_id HAdd));
+          return b
+        | HEvict ->
+          let b = ha_add v.hevict n t.serialization_buffer in
+          fold_epoch_hash_perm e v
+               (update_if b (Map.sel tsm.epoch_hashes e)
+                            (update_hash (Map.sel tsm.epoch_hashes e) r ts thread_id HEvict));
+          return b
+      in
+      EpochMap.ghost_put t.epoch_hashes e v _;
+      rewrite (EpochMap.perm _ _ _ _)
+              (EpochMap.full_perm t.epoch_hashes M.init_epoch_hash
+                           (Map.upd tsm.epoch_hashes e
+                                   (update_if b (Map.sel tsm.epoch_hashes e)
+                                                (update_hash (Map.sel tsm.epoch_hashes e) r ts thread_id ht))));
+      intro_exists _ (array_pts_to t.serialization_buffer);
+      maybe_update_epoch_hash_equiv b tsm e r ts thread_id ht;
+      rewrite (thread_state_inv_core t (maybe_update_epoch_hash b tsm e r ts thread_id ht))
+              (thread_state_inv_core t (update_if b tsm (update_epoch_hash tsm e r ts thread_id ht)));
+      return b
+#pop-options
+
+let vaddb (#tsm:M.thread_state_model)
+          (t:thread_state_t)
+          (s:slot_id)
+          (ts:timestamp)
+          (thread_id:T.thread_id)
+          (r:T.record)
+  : STT bool
+       (thread_state_inv_core t tsm)
+       (fun b -> thread_state_inv_core t (update_if b tsm (M.vaddb tsm s ts thread_id r)))
+  = let b = M.check_slot_bounds s in
+    if not b then (fail t; return true)
+    else (
+      let (k, v) = r in
+      if M.is_root_key k then (fail t; return true)
+      else (
+        let ropt = A.read t.store (as_u32 s) in
+        if Some? ropt then (fail t; return true) //slot is already full
+        else (
+          //add hash (k, v, t, thread_id) to hadd.[epoch_of_timestamp t]
+          let ok = update_ht t (M.epoch_of_timestamp ts) r ts thread_id HAdd in
+          if ok
+          then (
+             rewrite (thread_state_inv_core t _)
+                     (thread_state_inv_core t (update_epoch_hash tsm (M.epoch_of_timestamp ts) r ts thread_id HAdd));
+            let ts_opt = next ts in
+            match ts_opt with
+            | None -> fail t; return true
+            | Some t' ->
+              let clock = R.read t.clock in
+              let next_clock = max clock t' in
+              R.write t.clock next_clock;
+              A.write t.store (as_u32 s) (Some (M.mk_entry k v M.BAdd));
+              return true
+          )
+          else (
+            rewrite (thread_state_inv_core t _) (thread_state_inv_core t tsm);
+            return ok
+          )
+        )
+      )
+    )
+
+////////////////////////////////////////////////////////////////////////////////
+//vevictm
+////////////////////////////////////////////////////////////////////////////////
+
+let evict_from_store (#tsm:M.thread_state_model)
+                     (t:thread_state_t)
+                     (s:slot)
+                     (s':slot { M.has_slot tsm s' })
+                     (d:bool)
+  : STT unit
+    (thread_state_inv_core t tsm)
+    (fun _ -> thread_state_inv_core t (M.mevict_from_store tsm s s' d))
+  = let Some r' = A.read t.store (as_u32 s') in
+    let e' =
+        if d
+        then { r' with M.l_child_in_store = None }
+        else { r' with M.r_child_in_store = None }
+    in
+    A.write t.store (as_u32 s') (Some e');
+    A.write t.store (as_u32 s) None;
+    ()
+
+let vevictm (#tsm:M.thread_state_model)
+            (t:thread_state_t)
+            (s s':slot_id)
+  : STT unit
+    (thread_state_inv_core t tsm)
+    (fun _ -> thread_state_inv_core t (M.vevictm tsm s s'))
+  = if not (M.check_slot_bounds s)
+    || not (M.check_slot_bounds s')
+    then (R.write t.failed true; ())
+    else if s = s'
+    then (R.write t.failed true; ())
+    else (
+      let e = A.read t.store (as_u32 s) in
+      let e' = A.read t.store (as_u32 s') in
+      match e, e' with
+      | None, _
+      | _, None -> R.write t.failed true; ()
+      | Some r, Some r' ->
+        let gk = r.M.key in
+        let v = r.M.value in
+        let gk' = r'.M.key in
+        let v' = r'.M.value in
+        let k = M.to_base_key gk in
+        let k' = M.to_base_key gk' in
+        (* check k is a proper descendent of k' *)
+        if not (KU.is_proper_descendent k k')
+        then (R.write t.failed true; ())
+        (* check k does not have a (merkle) child in the store *)
+        else if entry_points_to_some_slot r true
+             ||  entry_points_to_some_slot r false
+        then (R.write t.failed true; ())
+        else (
+          let d = KU.desc_dir k k' in
+          let Some v' = M.to_merkle_value v' in
+          let dh' = M.desc_hash_dir v' d in
+          let h = M.hashfn v in
+          match dh' with
+          | T.Dh_vnone _ -> fail t; ()
+          | T.Dh_vsome {T.dhd_key=k2; T.dhd_h=h2; T.evicted_to_blum = b2} ->
+            if k2 <> k then (fail t; ())
+            else if Some? r.M.parent_slot &&
+                    (fst (Some?.v r.M.parent_slot) <> s' ||
+                     snd (Some?.v r.M.parent_slot) <> d)
+            then (fail t; ())
+            else if None? r.M.parent_slot
+                 && entry_points_to_some_slot r' d
+            then (fail t; ())
+            else (
+              let v'_upd = M.update_merkle_value v' d k h false in
+              update_value t s' (T.MValue v'_upd);
+              evict_from_store t s s' d;
+              ()
+            )
+        )
+      )
+
+////////////////////////////////////////////////////////////////////////////////
+//vevictb
+////////////////////////////////////////////////////////////////////////////////
+let sat_evictb_checks (#tsm:M.thread_state_model)
+                      (t:thread_state_t)
+                      (s:slot)
+                      (ts:timestamp)
+  : ST bool
+    (thread_state_inv_core t tsm)
+    (fun _ -> thread_state_inv_core t tsm)
+    (requires True)
+    (ensures fun b -> b == M.sat_evictb_checks tsm s ts)
+  = let ropt = A.read t.store (as_u32 s) in
+    match ropt with
+    | None ->
+      return false
+    | Some r ->
+      let k = r.key in
+      let v = r.value in
+      let clock = R.read t.clock in
+      let b =
+        not (M.is_root_key k) &&
+        (* check time of evict < current time *)
+        clock `M.timestamp_lt` ts &&
+        (* check k has no (merkle) children n the store *)
+        not (entry_points_to_some_slot r true) &&
+        not (entry_points_to_some_slot r false)
+      in
+      return b
+
+let vevictb_update_hash_clock (#tsm:M.thread_state_model)
+                              (t:thread_state_t)
+                              (s:slot)
+                              (ts:timestamp { M.sat_evictb_checks tsm s ts })
+   : ST bool
+     (thread_state_inv_core t tsm)
+     (fun b -> thread_state_inv_core t (update_if b tsm (M.vevictb_update_hash_clock tsm s ts)))
+     (requires tsm.thread_id == t.thread_id)
+     (ensures fun _ -> True)
+   = let Some r = A.read t.store (as_u32 s) in
+     let k = r.key in
+     let v = r.value in
+     (* update evict hash *)
+     let e = M.epoch_of_timestamp ts in
+     let b = update_ht t e (k, v) ts t.thread_id HEvict in
+     if b
+     then (
+       R.write t.clock ts;
+       return b
+     )
+     else (
+       rewrite (thread_state_inv_core t _) (thread_state_inv_core t tsm);
+       return b
+     )
+
+let vevictb (#tsm:M.thread_state_model)
+            (t:thread_state_t)
+            (s:slot_id)
+            (ts:timestamp)
+  : ST bool
+    (thread_state_inv_core t tsm)
+    (fun b -> thread_state_inv_core t (update_if b tsm (M.vevictb tsm s ts)))
+    (requires t.thread_id == tsm.thread_id)
+    (ensures fun _ -> True)
+  = let bounds_failed = not (M.check_slot_bounds s) in
+    if bounds_failed //not hoisting this leads to weirdness
+    then (
+      R.write t.failed true;
+      return true
+    )
+    else (
+      let b = sat_evictb_checks t s ts in
+      if not b
+      then (
+        fail t;
+        return true
+      )
+      else (
+        let Some r = A.read t.store (as_u32 s) in
+        if r.add_method <> M.BAdd
+        then (fail t; return true)
+        else (
+          let b = vevictb_update_hash_clock t s ts in
+          if b
+          then (
+            A.write t.store (as_u32 s) None;
+            return true
+          )
+          else (
+            rewrite (thread_state_inv_core t _)
+                    (thread_state_inv_core t tsm);
+            return false
+          )
+        )
+      )
+    )
+
+////////////////////////////////////////////////////////////////////////////////
+//vevictbm: A bit delicate. TODO should debug the SMT queries.
+////////////////////////////////////////////////////////////////////////////////
+
+let vevictbm (#tsm:M.thread_state_model)
+             (t:thread_state_t)
+             (s s':slot_id)
+             (ts:timestamp)
+  : ST bool
+    (thread_state_inv_core t tsm)
+    (fun b -> thread_state_inv_core t (update_if b tsm (M.vevictbm tsm s s' ts)))
+    (t.thread_id == tsm.thread_id)
+    (fun _ -> True)
+  = let bounds_failed =
+          not (M.check_slot_bounds s)
+        || not (M.check_slot_bounds s')
+    in
+    if bounds_failed then fail_as t _
+    else if s = s' then fail_as t _
+    else let se_checks = sat_evictb_checks t s ts in
+         if not se_checks then fail_as t _
+         else let ropt = A.read t.store (as_u32 s') in
+              match ropt with
+              | None -> fail_as t _
+              | Some r' ->
+                let Some r = A.read t.store (as_u32 s) in
+                if r.add_method <> M.MAdd
+                then (let b = fail_as t _ in return b)
+                else (
+                  let gk = r.key in
+                  let gk' = r'.key in
+                  let v' = r'.value in
+                  let k = M.to_base_key gk in
+                  let k' = M.to_base_key gk' in
+                  if not (KU.is_proper_descendent k k')
+                  then let b = fail_as t _ in return b
+                  else (
+                    let Some mv' = M.to_merkle_value v' in
+                    let d = KU.desc_dir k k' in
+                    let dh' = M.desc_hash_dir mv' d in
+                    match dh' returns
+                          (STT bool (thread_state_inv_core t tsm)
+                                    (fun b -> thread_state_inv_core t (update_if b tsm (M.vevictbm tsm s s' ts))))
+                    with
+                    | T.Dh_vnone _ ->
+                      let b = fail_as t _ in return b
+
+                    | T.Dh_vsome {T.dhd_key=k2;
+                                  T.dhd_h=h2;
+                                  T.evicted_to_blum = b2} ->
+                      if (k2 <> k) || (b2 = T.Vtrue)
+                      then let b = fail_as t _ in return b
+                      else if None? r.parent_slot
+                           || fst (Some?.v r.parent_slot) <> s'
+                           || snd (Some?.v r.parent_slot) <> d
+                      then let b = fail_as t _ in return b
+                      else (
+                        let b = vevictb_update_hash_clock t s ts in
+                        if b
+                        then (
+                          // rewrite (thread_state_inv_core t _)
+                          //         (thread_state_inv_core t (M.vevictb_update_hash_clock tsm s ts));
+                          let mv'_upd = M.update_merkle_value mv' d k h2 true in
+                          update_value t s' (MValue mv'_upd);
+                          evict_from_store t s s' d;
+                          return true
+                        )
+                        else (
+                          rewrite (thread_state_inv_core t _)
+                                  (thread_state_inv_core t tsm);
+                          return false
+                        ))))
+
+////////////////////////////////////////////////////////////////////////////////
+// nextepoch
+////////////////////////////////////////////////////////////////////////////////
+
+let new_epoch (e:M.epoch_id)
+  : STT EH.epoch_hashes_t
+    emp
+    (fun v -> EH.epoch_hash_perm e v M.init_epoch_hash)
+  = let hadd = HA.create () in
+    let hev = HA.create () in
+    let eh : EH.epoch_hashes_t = { hadd = hadd; hevict = hev } in
+    rewrite (HA.ha_val hadd _ `star` HA.ha_val hev _)
+            (EH.epoch_hash_perm e eh M.init_epoch_hash);
+    return eh
+
+
+let epoch_map_add (#v:Type0)
+               (#contents:Type0)
+               (#vp:M.epoch_id -> v -> contents -> vprop)
+               (#init:Ghost.erased contents)
+               (#m:Ghost.erased (EpochMap.repr contents))
+               (a:EpochMap.tbl vp)
+               (i:M.epoch_id)
+               (x:v)
+               (c:Ghost.erased contents)
+  : STT unit
+    (EpochMap.full_perm a init m `star`
+     vp i x c)
+    (fun _ ->
+      EpochMap.full_perm a init (Map.upd m i c))
+  = EpochMap.put a i x _;
+    assert (PartialMap.remove i (EpochMap.empty_borrows #v) `PartialMap.equal`
+            EpochMap.empty_borrows #v);
+    rewrite (EpochMap.perm a _ _ (PartialMap.remove i EpochMap.empty_borrows))
+            (EpochMap.full_perm a init (Map.upd m i c))
+
+let nextepoch (#tsm:M.thread_state_model)
+              (t:thread_state_t)
+  : STT unit
+    (thread_state_inv_core t tsm)
+    (fun _ -> thread_state_inv_core t (M.nextepoch tsm))
+  = let c = R.read t.clock in
+    let e = M.epoch_of_timestamp c in
+    let res = st_check_overflow_add32 e 1ul in //Ugh. need this wrapper, else weirdness
+    match res with
+    | None ->
+      fail t; ()
+    | Some nxt ->
+      let c = U64.shift_left (Cast.uint32_to_uint64 nxt) 32ul in
+      R.write t.clock c;
+      let eht = new_epoch nxt in
+      epoch_map_add t.epoch_hashes nxt eht M.init_epoch_hash;
+      ()
+
+////////////////////////////////////////////////////////////////////////////////
+//verify_epoch: One of the most delicate functions in the API is
+//verify_epoch, since it involves working with the aggregate epoch state
+////////////////////////////////////////////////////////////////////////////////
+
+let verify_epoch_committed_entries (tsm:M.thread_state_model)
+  : Lemma (requires
+             not tsm.failed /\
+             not (M.verifyepoch tsm).failed)
+          (ensures
+            (M.committed_entries (spec_verify_epoch tsm) ==
+            (spec_verify_epoch tsm).processed_entries))
+  = let tsm' = spec_verify_epoch tsm in
+    let _, last = Seq.un_snoc tsm'.processed_entries in
+    let is_verify = (function VerifyEpoch -> true | _ -> false) in
+    Zeta.SeqAux.lemma_last_index_correct2
+        is_verify
+        tsm'.processed_entries
+        (Seq.length tsm.processed_entries);
+    Zeta.SeqAux.lemma_fullprefix_equal tsm'.processed_entries
+
+let aggregate_one_epoch_hash (source:AEH.epoch_hashes_repr)
+                             (dest:AEH.epoch_hashes_repr)
+                             (e:M.epoch_id)
+  : AEH.epoch_hashes_repr
+  = Map.upd dest e (AEH.aggregate_epoch_hash
+                      (Map.sel dest e)
+                      (Map.sel source e))
+
+let aggregate_epoch_hash (b0 b1:bool) (e0 e1:M.epoch_hash)
+  : M.epoch_hash
+  = { hadd = update_if b0 e0.hadd (HA.aggregate_hashes e0.hadd e1.hadd);
+      hevict = update_if b1 e0.hevict (HA.aggregate_hashes e0.hevict e1.hevict) }
+
+
+let aggregate_epoch_hashes_t (#e:_)
+                             (#s #d:M.epoch_hash)
+                             (src:EH.epoch_hashes_t)
+                             (dst:EH.epoch_hashes_t)
+  : STT bool
+    (EH.epoch_hash_perm e src s `star`
+     EH.epoch_hash_perm e dst d)
+    (fun b ->
+      EH.epoch_hash_perm e src s `star`
+      (if b
+       then EH.epoch_hash_perm e dst (AEH.aggregate_epoch_hash d s)
+       else exists_ (EH.epoch_hash_perm e dst)))
+  = unfold_epoch_hash_perm e src s;
+    unfold_epoch_hash_perm e dst d;
+    let b = HA.aggregate dst.hadd src.hadd in
+    if b
+    then (
+      rewrite (HA.ha_val dst.hadd _)
+              (HA.ha_val dst.hadd (AEH.aggregate_epoch_hash d s).M.hadd);
+      let b = HA.aggregate dst.hevict src.hevict in
+      fold_epoch_hash_perm e src s;
+      if b
+      then (
+        rewrite (HA.ha_val dst.hevict _)
+                (HA.ha_val dst.hevict (AEH.aggregate_epoch_hash d s).M.hevict);
+        fold_epoch_hash_perm e dst (update_if true d (AEH.aggregate_epoch_hash d s));
+        return true
+      )
+      else (
+        let w : M.epoch_hash =
+          { hadd = (AEH.aggregate_epoch_hash d s).M.hadd;
+            hevict = d.hevict }
+        in
+        rewrite (HA.ha_val dst.hadd _)
+                (HA.ha_val dst.hadd w.hadd);
+        rewrite (HA.ha_val dst.hevict _)
+                (HA.ha_val dst.hevict w.hevict);
+        fold_epoch_hash_perm e dst w;
+        intro_exists w (EH.epoch_hash_perm e dst);
+        return false
+      )
+    )
+    else (
+      fold_epoch_hash_perm e src s;
+      rewrite (HA.ha_val dst.hadd _)
+              (HA.ha_val dst.hadd d.hadd);
+      fold_epoch_hash_perm e dst d;
+      intro_exists d (EH.epoch_hash_perm e dst);
+      return false
+    )
+
+inline_for_extraction
+let with_value_of_key (#v:Type0)
+                      (#contents:Type0)
+                      (#vp: M.epoch_id -> v -> contents -> vprop)
+                      (#init: erased contents)
+                      (#m:erased (EpochMap.repr contents))
+                      (#cf:contents -> GTot contents)
+                      (t:EpochMap.tbl vp)
+                      (i:M.epoch_id)
+                      ($f: (value:v -> STT unit
+                                         (vp i value (Map.sel m i))
+                                         (fun _ -> vp i value (cf (Map.sel m i)))))
+  : STT bool
+    (EpochMap.full_perm t init m)
+    (fun b -> EpochMap.full_perm t init (update_if b (reveal m) (Map.upd m i (cf (Map.sel m i)))))
+  = let res = EpochMap.get t i in
+    match res with
+    | EpochMap.Found value ->
+      rewrite (EpochMap.get_post _ _ _ _ _ _)
+              (EpochMap.perm t init m (PartialMap.upd i value EpochMap.empty_borrows) `star`
+               vp i value (Map.sel m i));
+      f value;
+      EpochMap.ghost_put t i value _;
+      return true
+    | _ ->
+      rewrite (EpochMap.get_post _ _ _ _ _ _)
+              (EpochMap.full_perm t init m);
+      return false
+
+/// Updates the aggregate epoch hash for a thread with the
+/// t thread-local epoch hashes for epoch e
+let rec propagate_epoch_hash (#tsm:M.thread_state_model)
+                             (t:thread_state_t)
+                             (#hv:erased AEH.epoch_hashes_repr)
+                             (hashes : AEH.all_epoch_hashes)
+                             (e:M.epoch_id)
+  : STT bool
+    (thread_state_inv_core t tsm `star`
+     EpochMap.full_perm hashes M.init_epoch_hash hv)
+    (fun b ->
+      thread_state_inv_core t tsm `star`
+      (if b
+       then EpochMap.full_perm hashes M.init_epoch_hash (aggregate_one_epoch_hash (spec_verify_epoch tsm).epoch_hashes hv e)
+       else exists_ (EpochMap.full_perm hashes M.init_epoch_hash)))
+  = let dst = EpochMap.get hashes e in
+    match dst with
+    | EpochMap.NotFound ->
+      rewrite (EpochMap.get_post _ _ _ _ _ _)
+              (EpochMap.full_perm hashes M.init_epoch_hash hv);
+      intro_exists_erased hv (EpochMap.full_perm hashes M.init_epoch_hash);
+      return false
+
+    | EpochMap.Fresh ->
+      rewrite (EpochMap.get_post _ _ _ _ _ _)
+              (EpochMap.full_perm hashes M.init_epoch_hash hv);
+      let eh = new_epoch e in
+      epoch_map_add hashes e eh _;
+      let b = propagate_epoch_hash t hashes e in
+      if b then (
+        rewrite (if b then _ else _)
+                (EpochMap.full_perm hashes M.init_epoch_hash
+                                    (aggregate_one_epoch_hash (spec_verify_epoch tsm).epoch_hashes
+                                                              (Map.upd hv e M.init_epoch_hash)
+                                                              e));
+        assert (Map.sel hv e == M.init_epoch_hash);
+        assert (Map.upd hv e M.init_epoch_hash `Map.equal` reveal hv);
+        rewrite (EpochMap.full_perm hashes M.init_epoch_hash
+                                    (aggregate_one_epoch_hash (spec_verify_epoch tsm).epoch_hashes
+                                                              (Map.upd hv e M.init_epoch_hash)
+                                                              e))
+                (EpochMap.full_perm hashes M.init_epoch_hash
+                                    (aggregate_one_epoch_hash (spec_verify_epoch tsm).epoch_hashes
+                                                              hv
+                                                              e));
+        return true
+      ) else (
+        rewrite (if b then _ else _)
+                (exists_ (EpochMap.full_perm hashes M.init_epoch_hash));
+        return false
+      )
+
+    | EpochMap.Found dst ->
+
+      rewrite (EpochMap.get_post _ _ _ _ _ _)
+              (EpochMap.perm hashes M.init_epoch_hash hv (PartialMap.upd e dst EpochMap.empty_borrows) `star`
+               EH.epoch_hash_perm e dst (Map.sel hv e));
+      let src = EpochMap.get t.epoch_hashes e in
+      match src with
+      | EpochMap.NotFound
+      | EpochMap.Fresh ->
+        rewrite (EpochMap.get_post _ _ _ t.epoch_hashes _ _)
+                (EpochMap.full_perm t.epoch_hashes M.init_epoch_hash tsm.epoch_hashes);
+        EpochMap.ghost_put hashes e dst _;
+        intro_exists_erased hv (EpochMap.full_perm hashes M.init_epoch_hash);
+        return false
+
+      | EpochMap.Found src ->
+
+        rewrite (EpochMap.get_post _ _ _ _ _ _)
+                (EpochMap.perm t.epoch_hashes M.init_epoch_hash tsm.epoch_hashes (PartialMap.upd e src EpochMap.empty_borrows) `star`
+                 EH.epoch_hash_perm e src (Map.sel tsm.epoch_hashes e));
+        let b = aggregate_epoch_hashes_t src dst in
+        if b
+        then (
+          rewrite (if b then _ else _)
+                  (EH.epoch_hash_perm e dst (AEH.aggregate_epoch_hash
+                                               (Map.sel hv e)
+                                               (Map.sel tsm.epoch_hashes e)));
+          EpochMap.ghost_put t.epoch_hashes e src _; //this should be a ghost put
+          EpochMap.ghost_put hashes e dst _;
+          return true
+        )
+        else (
+          rewrite (if b then _ else _)
+                  (exists_ (EH.epoch_hash_perm e dst));
+          let vv = elim_exists #_ #_ #(EH.epoch_hash_perm e dst) () in
+          assert_ (EH.epoch_hash_perm e dst vv);
+          EpochMap.ghost_put t.epoch_hashes e src _; //this should be a ghost put
+          EpochMap.ghost_put hashes e dst _;
+          assert_ (EpochMap.full_perm hashes M.init_epoch_hash (Map.upd hv e vv));
+          intro_exists (Map.upd hv e vv) (EpochMap.full_perm hashes M.init_epoch_hash);
+          return false
+        )
+
+let update_bitmap_spec (bm:EpochMap.repr AEH.tid_bitmap)
+                       (e:M.epoch_id)
+                       (tid:tid)
+  : EpochMap.repr AEH.tid_bitmap
+  = Map.upd bm e (Seq.upd (Map.sel bm e) (U16.v tid) true)
+
+/// Update the bitmap for tid indicating that it's epoch contribution
+/// is ready
+let update_bitmap (#bm:erased _)
+                  (tid_bitmaps: AEH.epoch_tid_bitmaps)
+                  (e:M.epoch_id)
+                  (tid:tid)
+  : STT bool
+    (EpochMap.full_perm tid_bitmaps AEH.all_zeroes bm)
+    (fun b ->
+      EpochMap.full_perm tid_bitmaps AEH.all_zeroes
+                  (update_if b
+                             (reveal bm)
+                             (update_bitmap_spec bm e tid)))
+  = [@@inline_let]
+    let update_tid (v:larray bool n_threads)
+      : STT unit
+            (array_pts_to v (Map.sel bm e))
+            (fun _ -> array_pts_to v (Seq.upd (Map.sel bm e) (U16.v tid) true))
+      = A.write v (as_u32 tid) true;
+        ()
+    in
+    with_value_of_key tid_bitmaps e update_tid
+
+let update_logs_of_tid
+         (mlogs_v:AEH.all_processed_entries)
+         (tsm:M.thread_state_model)
+  : GTot AEH.all_processed_entries
+  = Seq.upd mlogs_v (U16.v tsm.thread_id) tsm.processed_entries
+
+let map_of_seq_update_lemma  (mlogs_v:AEH.all_processed_entries)
+                             (tsm:M.thread_state_model)
+  : Lemma (Map.equal (Map.upd (Map.upd (AEH.map_of_seq mlogs_v) tsm.thread_id None)
+                              tsm.thread_id
+                              (Some (spec_verify_epoch tsm).processed_entries))
+                     (AEH.map_of_seq (update_logs_of_tid mlogs_v (spec_verify_epoch tsm))))
+  = ()
+
+/// A key ghost step:
+///
+///   Update the thread local log and then propagate the updated to
+///   the anchored global state
+let commit_entries #o
+                   (#tsm:M.thread_state_model)
+                   (#mlogs_v:AEH.all_processed_entries)
+                   (t:thread_state_t)
+                   (mylogref:TLM.t)
+  : STGhost unit o
+     (TLM.tid_pts_to mylogref t.thread_id full tsm.processed_entries false `star`
+      TLM.global_anchor mylogref (AEH.map_of_seq mlogs_v) `star`
+      G.pts_to t.processed_entries full (M.verifyepoch tsm).processed_entries)
+     (fun _ ->
+      TLM.tid_pts_to mylogref t.thread_id full (spec_verify_epoch tsm).processed_entries false `star`
+      TLM.global_anchor mylogref (AEH.map_of_seq (update_logs_of_tid mlogs_v (spec_verify_epoch tsm))) `star`
+      G.pts_to t.processed_entries full (spec_verify_epoch tsm).processed_entries)
+     (requires
+       t.thread_id == tsm.thread_id /\
+       not tsm.failed /\
+       not (M.verifyepoch tsm).failed)
+     (ensures fun _ -> True)
+  = TLM.take_anchor_tid mylogref _ _ _ _;
+    verify_epoch_committed_entries tsm;
+    TLM.update_anchored_tid_log mylogref _ _ (spec_verify_epoch tsm).processed_entries;
+    TLM.put_anchor_tid mylogref _ _ _ _;
+    G.write t.processed_entries (spec_verify_epoch tsm).processed_entries;
+    map_of_seq_update_lemma mlogs_v tsm;
+    rewrite
+          (TLM.global_anchor mylogref _)
+          (TLM.global_anchor mylogref (AEH.map_of_seq (update_logs_of_tid mlogs_v (spec_verify_epoch tsm))))
+
+#push-options "--fuel 2"
+let spec_verify_epoch_entries_invariants (tsm:M.thread_state_model)
+  : Lemma
+    (requires not tsm.failed /\
+              not (spec_verify_epoch tsm).failed /\
+              tsm_entries_invariant tsm)
+    (ensures (tsm_entries_invariant (spec_verify_epoch tsm)))
+  = assert (tsm == M.verify_model (M.init_thread_state_model tsm.thread_id) tsm.processed_entries);
+    let tsm' = spec_verify_epoch tsm in
+    assert (tsm'.processed_entries == Seq.snoc tsm.processed_entries VerifyEpoch);
+    assert (Zeta.SeqAux.prefix tsm'.processed_entries
+                               (Seq.length tsm.processed_entries)
+            `Seq.equal`
+           tsm.processed_entries);
+    assert (tsm' == M.verify_model (M.init_thread_state_model tsm.thread_id) tsm'.processed_entries)
+#pop-options
+
+let last_verified_epoch_constant (tsm:M.thread_state_model)
+  : Lemma
+    (requires
+      tsm_entries_invariant tsm)
+    (ensures (
+      let tsm0 = M.verify_model (M.init_thread_state_model tsm.thread_id) (M.committed_entries tsm) in
+      tsm.last_verified_epoch == tsm0.last_verified_epoch))
+  = admit() //the last_verified_epoch only changed when processing a verify_epoch entry
+
+let advance_per_thread_bitmap_and_max  (bitmaps:EpochMap.repr AEH.tid_bitmap)
+                                       (max:_)
+                                       (mlogs_v:_)
+                                       (tsm:M.thread_state_model)
+                                       (e:M.epoch_id)
+  : Lemma
+    (requires (
+      let tsm' = spec_verify_epoch tsm in
+      AEH.per_thread_bitmap_and_max bitmaps max mlogs_v tsm.thread_id /\
+      tsm'.last_verified_epoch == e /\
+      not tsm'.failed /\
+      tsm_entries_invariant tsm /\
+      M.committed_entries tsm == AEH.log_of_tid mlogs_v tsm.thread_id
+      ))
+    (ensures (
+      let tsm' = spec_verify_epoch tsm in
+      let bitmaps' = update_bitmap_spec bitmaps e tsm.thread_id in
+      let logs' = update_logs_of_tid mlogs_v tsm' in
+      AEH.per_thread_bitmap_and_max bitmaps' max logs' tsm.thread_id))
+  = let log0 = AEH.log_of_tid mlogs_v tsm.thread_id in
+    let tsm0 = M.verify_model (M.init_thread_state_model tsm.thread_id) log0 in
+    last_verified_epoch_constant tsm;
+    assert (tsm0.last_verified_epoch == tsm.last_verified_epoch);
+    let tsm' = spec_verify_epoch tsm in
+    let bitmaps' = update_bitmap_spec bitmaps e tsm.thread_id in
+    let logs' = update_logs_of_tid mlogs_v tsm' in
+    spec_verify_epoch_entries_invariants tsm;
+    assert (U32.v max <= U32.v tsm0.last_verified_epoch);
+    assert (U32.v e == U32.v tsm.last_verified_epoch + 1);
+    assert (U32.v max <= U32.v tsm'.last_verified_epoch)
+
+let restore_all_threads_bitmap_and_max  (bitmaps:AEH.epoch_bitmaps_repr)
+                                        (max:_)
+                                        (mlogs_v:_)
+                                        (tsm:M.thread_state_model)
+                                        (e:M.epoch_id)
+  : Lemma
+    (requires
+      (let tsm' = spec_verify_epoch tsm in
+       (forall tid. AEH.per_thread_bitmap_and_max bitmaps max mlogs_v tid) /\
+       tsm'.last_verified_epoch = e /\
+       tsm_entries_invariant tsm /\
+       not tsm'.failed /\
+       M.committed_entries tsm == AEH.log_of_tid mlogs_v tsm.thread_id))
+    (ensures
+      (let tsm' = spec_verify_epoch tsm in
+        (forall tid. AEH.per_thread_bitmap_and_max
+                      (update_bitmap_spec bitmaps e tsm.thread_id)
+                      max
+                      (update_logs_of_tid mlogs_v tsm')
+                      tid)))
+  = advance_per_thread_bitmap_and_max bitmaps max mlogs_v tsm e
+#push-options "--print_implicits --print_bound_var_types"
+let lemma_restore_hashes_bitmaps_max_ok
+                                  (hashes:AEH.epoch_hashes_repr)
+                                  (bitmaps:AEH.epoch_bitmaps_repr)
+                                  (max:M.epoch_id)
+                                  (mlogs_v:AEH.all_processed_entries)
+                                  (tsm:M.thread_state_model)
+                                  (e:M.epoch_id)
+  : Lemma
+    (requires
+      (spec_verify_epoch tsm).last_verified_epoch = e /\
+      AEH.hashes_bitmaps_max_ok hashes bitmaps max mlogs_v /\
+      tsm_entries_invariant tsm /\
+      not (spec_verify_epoch tsm).failed /\
+      M.committed_entries tsm == AEH.log_of_tid mlogs_v tsm.thread_id)
+    (ensures (
+      let tsm' = spec_verify_epoch tsm in
+      let hashes' = aggregate_one_epoch_hash tsm'.epoch_hashes hashes e in
+      let bitmaps' = update_bitmap_spec bitmaps e tsm'.thread_id in
+      let mlogs_v' = update_logs_of_tid mlogs_v tsm' in
+      AEH.hashes_bitmaps_max_ok hashes' bitmaps' max mlogs_v'))
+  = let log0 = AEH.log_of_tid mlogs_v tsm.thread_id in
+    let tsm0 = M.verify_model (M.init_thread_state_model tsm.thread_id) log0 in
+    let tsm' = spec_verify_epoch tsm in
+    let hashes' = aggregate_one_epoch_hash tsm'.epoch_hashes hashes e in
+    let bitmaps' = update_bitmap_spec bitmaps e tsm'.thread_id in
+    let mlogs_v' = update_logs_of_tid mlogs_v tsm' in
+    advance_per_thread_bitmap_and_max bitmaps max mlogs_v tsm e;
+    introduce forall (e':M.epoch_id).
+      Map.sel hashes' e' == AEH.aggregate_all_threads_epoch_hashes e' mlogs_v'
+    with (
+      if e = e'
+      then (
+        calc (==) {
+         AEH.aggregate_all_threads_epoch_hashes e mlogs_v';
+         (==) { _ by FStar.Tactics.(trefl()) }
+         Zeta.SeqAux.reduce #(AEH.epoch_hashes_repr) M.init_epoch_hash
+                       (fun s -> AEH.aggregate_epoch_hash (Map.sel s e))
+                       (AEH.all_threads_epoch_hashes_of_logs mlogs_v');
+         (==) {admit()} //probably easier to do this using the permutation monoid
+                             //and we need to know that the bit for tsm was false initially
+         AEH.aggregate_epoch_hash (AEH.aggregate_all_threads_epoch_hashes e mlogs_v)
+                                  (Map.sel tsm'.epoch_hashes e);
+        }
+      )
+      else (
+        assert (Map.sel hashes' e' == Map.sel hashes e');
+        assert (Map.sel hashes e' == AEH.aggregate_all_threads_epoch_hashes e' mlogs_v);
+        //need a framing lemma here
+        // -- we only updated the logs of tsm'
+        // -- the only epoch that was propagated was e, since mlogs_v contained all prior committed epoch
+        // -- so, only the epoch contents of e changed, not e'
+        assume (AEH.aggregate_all_threads_epoch_hashes e' mlogs_v ==
+                AEH.aggregate_all_threads_epoch_hashes e' mlogs_v')
+      )
+    );
+    assert (U32.v max <= U32.v tsm0.last_verified_epoch);
+    last_verified_epoch_constant tsm
+
+let restore_hashes_bitmaps_max_ok (#o:_)
+                                  (#hashes:AEH.epoch_hashes_repr)
+                                  (#bitmaps:AEH.epoch_bitmaps_repr)
+                                  (#max:M.epoch_id)
+                                  (#mlogs_v:AEH.all_processed_entries)
+                                  (tsm:M.thread_state_model)
+                                  (e:M.epoch_id)
+  : STGhost unit o
+    (pure (AEH.hashes_bitmaps_max_ok hashes bitmaps max mlogs_v))
+    (fun _ ->
+      let tsm' = spec_verify_epoch tsm in
+      let hashes' = aggregate_one_epoch_hash tsm'.epoch_hashes hashes e in
+      let bitmaps' = update_bitmap_spec bitmaps e tsm'.thread_id in
+      let mlogs_v' = update_logs_of_tid mlogs_v tsm' in
+      pure (AEH.hashes_bitmaps_max_ok hashes' bitmaps' max mlogs_v'))
+    (requires
+          M.committed_entries tsm == AEH.log_of_tid mlogs_v tsm.thread_id /\
+          (spec_verify_epoch tsm).last_verified_epoch = e /\
+          tsm_entries_invariant tsm /\
+          not (spec_verify_epoch tsm).failed)
+    (ensures fun _ -> True)
+  = elim_pure _;
+    lemma_restore_hashes_bitmaps_max_ok hashes bitmaps max mlogs_v tsm e;
+    intro_pure _
+
+////////////////////////////////////////////////////////////////////////////////
+// Finally verify_epoch itself
+////////////////////////////////////////////////////////////////////////////////
+let verify_epoch_core
+                 (#tsm:M.thread_state_model)
+                 (t:thread_state_t)
+                 (hashes : AEH.all_epoch_hashes)
+                 (tid_bitmaps : AEH.epoch_tid_bitmaps)
+                 (max_certified_epoch : R.ref M.epoch_id)
+                 (mlogs: TLM.t)
+                 (lock: cancellable_lock (AEH.lock_inv hashes tid_bitmaps max_certified_epoch mlogs))
+  : ST bool
+    (thread_state_inv_core t tsm `star`
+     TLM.tid_pts_to mlogs t.thread_id full tsm.processed_entries false)
+    (fun b ->
+      thread_state_inv_core t (update_if b tsm (spec_verify_epoch tsm)) `star`
+      TLM.tid_pts_to mlogs t.thread_id full (update_if b tsm.processed_entries
+                                                         (spec_verify_epoch tsm).processed_entries)
+                                            false)
+    (requires
+      t.thread_id == tsm.thread_id /\
+      tsm_entries_invariant tsm /\
+      not tsm.failed)
+    (ensures fun _ -> True)
+  = let e = R.read t.last_verified_epoch in
+    let e' = st_check_overflow_add32 e 1ul in
+    match e' with
+    | None ->
+      R.write t.failed true; return true
+
+    | Some e ->
+
+      let acquired = acquire lock in
+      if not acquired
+      then (
+        rewrite (maybe_acquired _ _)
+                emp;
+        return false
+      )
+      else (
+        rewrite (maybe_acquired _ _)
+                (AEH.lock_inv hashes tid_bitmaps max_certified_epoch mlogs `star` can_release lock);
+
+        let _hv = elim_exists () in
+        let _bitmaps = elim_exists () in
+        let _max = elim_exists () in
+        let _mlogs_v =
+          elim_exists #_ #_
+            #(AEH.lock_inv_body hashes tid_bitmaps max_certified_epoch mlogs
+                                _hv _bitmaps _max)
+            ()
+        in
+
+        TLM.extract_anchor_invariant mlogs _ _ _ _;
+        let b0 = propagate_epoch_hash t hashes e in
+        let b1 = update_bitmap tid_bitmaps e t.thread_id in
+        if not b0 || not b1
+        then ( //propagation failed, e.g., due to overflow
+           cancel lock;
+           drop _; //drop resources protected by lock; invariant is lost
+           return false
+        )
+        else (
+           R.write t.last_verified_epoch e;
+           assert_ (thread_state_inv_core t (M.verifyepoch tsm));
+           assert ((spec_verify_epoch tsm).last_verified_epoch == e);
+           commit_entries t mlogs;
+           restore_hashes_bitmaps_max_ok tsm e;
+           rewrite (if b0 then _ else _)
+                   (EpochMap.full_perm hashes M.init_epoch_hash (aggregate_one_epoch_hash (spec_verify_epoch tsm).epoch_hashes _hv e));
+           AEH.release_lock #(hide (aggregate_one_epoch_hash (spec_verify_epoch tsm).epoch_hashes _hv e))
+                            #(hide (update_bitmap_spec _bitmaps e (spec_verify_epoch tsm).thread_id))
+                            lock;
+           return true
+        )
+      )
+
+////////////////////////////////////////////////////////////////////////////////
+
+#push-options "--fuel 2 --z3rlimit_factor 4"
+let verify_epoch_inv (b:bool)
+                     (tsm:M.thread_state_model)
+  : Lemma
+    (requires tsm_entries_invariant tsm /\
+              not tsm.failed)
+    (ensures tsm_entries_invariant (update_if b tsm (spec_verify_epoch tsm)))
+  = let tsm' = update_if b tsm (spec_verify_epoch tsm) in
+    assert (tsm == M.verify_model (M.init_thread_state_model tsm.thread_id) tsm.M.processed_entries);
+    assert (Zeta.SeqAux.prefix tsm'.M.processed_entries (Seq.length tsm.M.processed_entries) `Seq.equal` tsm.M.processed_entries)
+#pop-options
+
+let verify_epoch (#tsm:M.thread_state_model)
+                 (t:thread_state_t)
+                 (aeh:AEH.aggregate_epoch_hashes)
+  : ST bool
+    (thread_state_inv t tsm `star`
+     TLM.tid_pts_to aeh.mlogs tsm.thread_id full tsm.processed_entries false)
+    (fun b ->
+      thread_state_inv t (update_if b tsm (spec_verify_epoch tsm)) `star`
+      TLM.tid_pts_to aeh.mlogs tsm.thread_id full
+                         (update_if b tsm.processed_entries
+                                      (spec_verify_epoch tsm).processed_entries)
+                         false)
+    (requires not tsm.failed)
+    (ensures fun _ -> True)
+  = elim_thread_state_inv #_ #tsm t;
+    rewrite (TLM.tid_pts_to _ _ _ _ _)
+            (TLM.tid_pts_to aeh.mlogs t.thread_id full tsm.processed_entries false);
+    let b = verify_epoch_core t aeh.hashes aeh.tid_bitmaps aeh.max_certified_epoch aeh.mlogs aeh.lock in
+    rewrite (TLM.tid_pts_to _ _ _ _ _)
+            (TLM.tid_pts_to aeh.mlogs tsm.thread_id full (update_if b tsm.processed_entries
+                                                                    (spec_verify_epoch tsm).processed_entries) false);
+    let tsm' = update_if b tsm (spec_verify_epoch tsm) in
+    verify_epoch_inv b tsm;
+    intro_thread_state_inv t;
+    return b
