steel/Zeta.Steel.VerifierSteps.fsti
@@ -1,0 +1,91 @@
+module Zeta.Steel.VerifierSteps
+include Zeta.Steel.VerifierTypes
+open FStar.Ghost
+open Steel.ST.Util
+open Zeta.Steel.ApplicationTypes
+open Zeta.Steel.FormatsManual
+open Zeta.Steel.Util
+module M = Zeta.Steel.ThreadStateModel
+module T = Zeta.Steel.FormatsManual
+#push-options "--ide_id_info_off"
+
+val create (tid:tid)
+  : STT thread_state_t
+    emp
+    (fun t -> thread_state_inv t (M.init_thread_state_model tid))
+
+val vaddm (#tsm:M.thread_state_model)
+          (t:thread_state_t)
+          (s s':slot_id)
+          (r:T.record)
+  : STT bool
+    (thread_state_inv_core t tsm)
+    (fun b ->
+      thread_state_inv_core t
+           (update_if b tsm (M.vaddm tsm s s' r)))
+
+val vaddb (#tsm:M.thread_state_model)
+          (t:thread_state_t)
+          (s:slot_id)
+          (ts:timestamp)
+          (thread_id:T.thread_id)
+          (r:T.record)
+  : STT bool
+       (thread_state_inv_core t tsm)
+       (fun b ->
+         thread_state_inv_core t
+               (update_if b tsm (M.vaddb tsm s ts thread_id r)))
+
+val vevictm (#tsm:M.thread_state_model)
+            (t:thread_state_t)
+            (s s':slot_id)
+  : STT unit
+    (thread_state_inv_core t tsm)
+    (fun _ -> thread_state_inv_core t (M.vevictm tsm s s'))
+
+val vevictb (#tsm:M.thread_state_model)
+            (t:thread_state_t)
+            (s:slot_id)
+            (ts:timestamp)
+  : ST bool
+    (thread_state_inv_core t tsm)
+    (fun b -> thread_state_inv_core t (update_if b tsm (M.vevictb tsm s ts)))
+    (requires VerifierTypes.thread_id t == tsm.thread_id)
+    (ensures fun _ -> True)
+
+val vevictbm (#tsm:M.thread_state_model)
+             (t:thread_state_t)
+             (s s':slot_id)
+             (ts:timestamp)
+  : ST bool
+    (thread_state_inv_core t tsm)
+    (fun b -> thread_state_inv_core t (update_if b tsm (M.vevictbm tsm s s' ts)))
+    (VerifierTypes.thread_id t == tsm.thread_id)
+    (fun _ -> True)
+
+val nextepoch (#tsm:M.thread_state_model)
+              (t:thread_state_t)
+  : STT unit
+    (thread_state_inv_core t tsm)
+    (fun _ -> thread_state_inv_core t (M.nextepoch tsm))
+
+module AEH = Zeta.Steel.AggregateEpochHashes
+module TLM = Zeta.Steel.ThreadLogMap
+let spec_verify_epoch (tsm:M.thread_state_model)
+  = let tsm = M.verifyepoch tsm in
+    if tsm.failed then tsm
+    else { tsm with M.processed_entries = Seq.snoc tsm.processed_entries (VerifyEpoch)}
+
+val verify_epoch (#tsm:M.thread_state_model)
+                 (t:thread_state_t)
+                 (aeh:AEH.aggregate_epoch_hashes)
+  : ST bool
+    (thread_state_inv t tsm `star`
+     TLM.tid_pts_to aeh.mlogs tsm.thread_id full tsm.processed_entries false)
+    (fun b ->
+      thread_state_inv t (update_if b tsm (spec_verify_epoch tsm)) `star`
+      TLM.tid_pts_to aeh.mlogs tsm.thread_id full (update_if b tsm.processed_entries
+                                                         (spec_verify_epoch tsm).processed_entries)
+                                            false)
+    (requires not tsm.failed)
+    (ensures fun _ -> True)
